Fix map_simpl

theories/map_simpl.v
@@ -8,52 +8,52 @@ Section simpl_gmap.
   Hypothesis HcountK: Countable K.
 
   (* reified gmap *)
-  Inductive rgmap {A M: Type}: Type :=
+  Inductive rgmap {A: Type}: Type :=
   | Ins (k: K) (a: A) (m: rgmap)
   | Del (k: K) (m: rgmap)
-  | Symb (m: M).
+  | Symb.
 
-  Fixpoint denote {A: Type} (rm: @rgmap A (gmap K A)): gmap K A :=
+  Fixpoint denote {A: Type} (rm: @rgmap A) (m: gmap K A): gmap K A :=
     match rm with
-    | Ins k a rm => <[k := a]> (denote rm)
-    | Del k rm => delete k (denote rm)
-    | Symb m => m
+    | Ins k a rm => <[k := a]> (denote rm m)
+    | Del k rm => delete k (denote rm m)
+    | Symb => m
     end.
 
-  Fixpoint rlength {A M: Type} (rm: @rgmap A M): nat :=
+  Fixpoint rlength {A: Type} (rm: @rgmap A): nat :=
     match rm with
     | Ins _ _ rm => S (rlength rm)
     | Del _ rm => S (rlength rm)
-    | Symb m => O
+    | Symb => O
     end.
 
-  Fixpoint remove_key {A M: Type} (k: K) (rm: @rgmap A M) :=
+  Fixpoint remove_key {A: Type} (k: K) (rm: @rgmap A) :=
     match rm with
     | Ins k' a rm => if decide (k = k') then remove_key k rm else Ins k' a (remove_key k rm)
     | Del k' rm => if decide (k = k') then remove_key k rm else Del k' (remove_key k rm)
-    | Symb m => Symb m
+    | Symb => Symb
     end.
 
   Lemma rlength_remove_key:
-    forall A M k (rm: @rgmap A M), rlength (remove_key k rm) <= rlength rm.
+    forall A k (rm: @rgmap A), rlength (remove_key k rm) <= rlength rm.
   Proof.
     induction rm; simpl; auto.
     - destruct (decide (k = k0)); simpl; lia.
     - destruct (decide (k = k0)); simpl; lia.
   Qed.
 
-  Equations simpl_rmap {A M: Type} (rm: @rgmap A M): @rgmap A M by wf (rlength rm) lt :=
+  Equations simpl_rmap {A: Type} (rm: @rgmap A): @rgmap A by wf (rlength rm) lt :=
     simpl_rmap (Ins k a rm) := Ins k a (simpl_rmap (remove_key k rm));
     simpl_rmap (Del k rm) := Del k (simpl_rmap (remove_key k rm));
-    simpl_rmap (Symb m) := Symb m.
+    simpl_rmap (Symb) := Symb.
   Next Obligation.
-    generalize (rlength_remove_key _ _ k rm). lia. Qed.
+    generalize (rlength_remove_key _ k rm). lia. Qed.
   Next Obligation.
-    generalize (rlength_remove_key _ _ k rm). lia. Qed.
+    generalize (rlength_remove_key _ k rm). lia. Qed.
 
   Lemma denote_remove_key_ins:
-    forall A (rm: @rgmap A (gmap K A)) k a,
-      <[k:=a]> (denote rm) = <[k:=a]> (denote (remove_key k rm)).
+    forall A (rm: @rgmap A) k a (m: gmap K A),
+      <[k:=a]> (denote rm m) = <[k:=a]> (denote (remove_key k rm) m).
   Proof.
     induction rm; simpl; auto.
     - intros. destruct (decide (k0 = k)).
@@ -67,8 +67,8 @@ Section simpl_gmap.
   Qed.
 
   Lemma denote_remove_key_del:
-    forall A (rm: @rgmap A (gmap K A)) k,
-      delete k (denote rm) = delete k (denote (remove_key k rm)).
+    forall A (rm: @rgmap A) k (m: gmap K A),
+      delete k (denote rm m) = delete k (denote (remove_key k rm) m).
   Proof.
     induction rm; simpl; auto.
     - intros. destruct (decide (k0 = k)).
@@ -82,9 +82,9 @@ Section simpl_gmap.
   Qed.
 
   Lemma simpl_rmap_correct':
-    forall A n (rm: @rgmap A (gmap K A)),
+    forall A n (rm: @rgmap A) (m: gmap K A),
       rlength rm <= n ->
-      denote rm = denote (simpl_rmap rm).
+      denote rm m = denote (simpl_rmap rm) m.
   Proof.
     induction n; intros.
     - destruct rm; simpl in H; try lia.
@@ -93,17 +93,17 @@ Section simpl_gmap.
       + rewrite simpl_rmap_equation_1; simpl.
         rewrite <- (IHn (remove_key k rm)).
         * apply denote_remove_key_ins.
-        * generalize (rlength_remove_key _ _ k rm). simpl in H; lia.
+        * generalize (rlength_remove_key _ k rm). simpl in H; lia.
       + rewrite simpl_rmap_equation_2; simpl.
         rewrite <- (IHn (remove_key k rm)).
         * apply denote_remove_key_del.
-        * generalize (rlength_remove_key _ _ k rm). simpl in H; lia.
+        * generalize (rlength_remove_key _ k rm). simpl in H; lia.
   Qed.
 
   Lemma simpl_rmap_correct:
-    forall A (rm rm': @rgmap A (gmap K A)),
+    forall A (rm rm': @rgmap A) (m: gmap K A),
       simpl_rmap rm = rm' ->
-      denote rm = denote rm'.
+      denote rm m = denote rm' m.
   Proof.
     intros. subst rm'. apply (simpl_rmap_correct' _ (rlength rm)); auto; lia.
   Qed.
@@ -115,10 +115,10 @@ From Ltac2 Require Import Ltac2 Option Constr.
 Ltac2 rec reify_helper kk aa term :=
   lazy_match! term with
   | <[?k := ?a]> ?m => let (rm, h) := reify_helper kk aa m in
-                      (constr:(@Ins $kk $aa (gmap $kk $aa) $k $a $rm), h)
+                      (constr:(@Ins $kk $aa $k $a $rm), h)
   | delete ?k ?m => let (rm, h) := reify_helper kk aa m in
-                   (constr:(@Del $kk $aa (gmap $kk $aa) $k $rm), h)
-  | ?m => (constr:(@Symb $kk $aa (gmap $kk $aa) $m), m)
+                   (constr:(@Del $kk $aa $k $rm), h)
+  | ?m => (constr:(@Symb $kk $aa), m)
 end.
 
 Local Ltac2 replace_with (lhs: constr) (rhs: constr) :=
@@ -127,30 +127,30 @@ Local Ltac2 replace_with (lhs: constr) (rhs: constr) :=
 Goal <[5 := 2]> (<[5 := 3]> (∅: gmap nat nat)) = <[5 := 2]> (∅: gmap nat nat).
   lazy_match! goal with
   | [|- ?x = _] => let (x', m) := reify_helper 'nat 'nat x in
-                 replace_with x '(@denote _ _ _ _ $x') > [() | reflexivity];
-                 let id := Option.get (Ident.of_string "x") in
-                 let h := Fresh.in_goal id in
-                 remember $m as $h;
-                 erewrite (@simpl_rmap_correct) > [() | vm_compute; subst $h; reflexivity];
-                 cbn [denote]; subst $h
+                 replace_with x '(@denote _ _ _ _ $x' $m) > [() | reflexivity];
+                 (* let id := Option.get (Ident.of_string "x") in *)
+                 (* let h := Fresh.in_goal id in *)
+                 (* remember $m as $h; *)
+                 erewrite (@simpl_rmap_correct) > [() | vm_compute; reflexivity];
+                 cbn [denote]
   end.
   reflexivity.
 Qed.
 
 Ltac2 map_simpl_aux k a x :=
-  Message.print (Message.of_string "Coucou");
-  let (x', m) := reify_helper k a x in
-  Message.print (Message.of_string "Coucou");
+  Message.print (Message.of_string "Reification Start");
+  let (x', m) := time (reify_helper k a x) in
+  Message.print (Message.of_string "Reification End");
   (* Message.print (Message.of_constr a); *)
   (* Message.print (Message.of_constr x); *)
   (* Message.print (Message.of_constr x'); *)
   (* Message.print (Message.of_constr '(@denote _ _ _ _ $x')); *)
-  replace_with x '(@denote _ _ _ _ $x') > [() | reflexivity];
-  let id := Option.get (Ident.of_string "x") in
-  let h := Fresh.in_goal id in
-  remember $m as $h;
-  erewrite (simpl_rmap_correct) > [() | Message.print (Message.of_string "Coucou"); vm_compute; Message.print (Message.of_string "Coucou"); subst $h; reflexivity];
-  cbn [denote]; subst $h.
+  replace_with x '(@denote _ _ _ _ $x' $m) > [() | reflexivity];
+  (* let id := Option.get (Ident.of_string "x") in *)
+  (* let h := Fresh.in_goal id in *)
+  (* remember $m as $h; *)
+  time (erewrite (simpl_rmap_correct)) > [() | Message.print (Message.of_string "End erewrite"); time vm_compute; Message.print (Message.of_string "End vm_compute"); time reflexivity];
+  time (cbn [denote]).
 
 From iris.proofmode Require Import environments.
 
