theories/map_simpl_test.v
@@ -5,7 +5,7 @@ Section test.
   Context `{memG Σ, regG Σ}.
 
   Lemma foo (w1 w2 w3: Word) :
-    ([∗ map] k↦y ∈ (<[r_t1:=w1]> (<[r_t2:=w2]> (<[r_t1:=w3]> ∅))), k ↦ᵣ y) -∗
+    ([∗ map] k↦y ∈ delete r_t2 (<[r_t1:=w1]> (<[r_t2:=w2]> (<[r_t1:=w3]> ∅))), k ↦ᵣ y) -∗
     r_t1 ↦ᵣ w1 ∗ r_t2 ↦ᵣ w2.
   Proof.
     iIntros "H".
